cfrontend/Csem.v
@@ -826,13 +826,14 @@ End SEMANTICS.
   without arguments and with an empty continuation. *)
 
 Inductive initial_state (p: program): state -> Prop :=
-  | initial_state_intro: forall b f m0,
+  | initial_state_intro: forall b f m0 m1 b0,
       let ge := globalenv p in
       Genv.init_mem p = Some m0 ->
       Genv.find_symbol ge p.(prog_main) = Some b ->
       Genv.find_funct_ptr ge b = Some f ->
       type_of_fundef f = Tfunction Tnil type_int32s cc_default ->
-      initial_state p (Callstate f nil Kstop m0 p.(prog_main)).
+      Mem.alloc m0 0 0 = (m1,b0) ->
+      initial_state p (Callstate f nil Kstop m1 p.(prog_main)).
 
 (** A final state is a [Returnstate] with an empty continuation. *)
 
